much better recursive scheme

dev2015/fsub0.v
@@ -633,6 +633,7 @@ Proof.
   unfold index. unfold index in H. rewrite H. rewrite E. rewrite EX. reflexivity.
 Qed.
 
+
 Lemma indexr_extend : forall X vs n n' x (T: X),
                        indexr n vs = Some T ->
                        indexr n ((n',x)::vs) = Some T.
@@ -950,228 +951,99 @@ Proof.
     rewrite IHGH0. reflexivity. assumption.
 Qed.
 
-Lemma stp2_extend_wip : forall G1 G2 T1 T2 H,
-                      stp2 G1 T1 G2 T2 H ->
-                      (forall x v, fresh G1 <= x ->
-                       stp2 ((x,v)::G1) T1 G2 T2 H) /\
-                      (forall x v, fresh G2 <= x ->
-                       stp2 G1 T1 ((x,v)::G2) T2 H) /\
-                      (forall x0 G0 T0 x1 v1 GH0 GH1, H=GH0++(x0, (G0, T0))::GH1 ->
-                       fresh G0 <= x1 ->
-                       stp2 G1 T1 G2 T2 (GH0++(x0, (((x1,v1)::G0), T0))::GH1)) /\
-                      (forall x0 G0 T0 x1 v1 x v GH0 GH1, H=GH0++(x0, (G0, T0))::GH1 ->
-                       fresh G1 <= x ->
-                       fresh G0 <= x1 ->
-                       stp2 ((x,v)::G1) T1 G2 T2 (GH0++(x0, (((x1,v1)::G0), T0))::GH1)) /\
-                      (forall x0 G0 T0 x1 v1 x v GH0 GH1, H=GH0++(x0, (G0, T0))::GH1 ->
-                       fresh G2 <= x ->
-                       fresh G0 <= x1 ->
-                       stp2 G1 T1 ((x,v)::G2) T2 (GH0++(x0, (((x1,v1)::G0), T0))::GH1)) /\
-                      (forall x0 G0 T0 x1 v1 x v x' v' GH0 GH1, H=GH0++(x0, (G0, T0))::GH1 ->
-                       fresh G1 <= x ->
-                       fresh G2 <= x' ->
-                       fresh G0 <= x1 ->
-                       stp2 ((x,v)::G1) T1 ((x',v')::G2) T2 (GH0++(x0, (((x1,v1)::G0), T0))::GH1)).
+Inductive venv_ext : venv -> venv -> Prop :=
+| venv_same : forall G, venv_ext G G
+| venv_cons : forall x T G1 G2, fresh G1 <= x -> venv_ext G1 G2 -> venv_ext ((x,T)::G1) G2.
+
+Inductive aenv_ext : aenv -> aenv -> Prop :=
+| aenv_nil : aenv_ext nil nil
+| aenv_cons : forall x T G' G A A', aenv_ext A' A -> venv_ext G' G -> aenv_ext ((x,(G',T))::A') ((x,(G,T))::A).
+
+Lemma index_extend_mult : forall G G' x T,
+                       index x G = Some T ->
+                       venv_ext G' G ->
+                       index x G' = Some T.
 Proof.
-  intros.
-  induction H0; split; try split; try split; try split; try split; intros; eauto;
-  try solve [inversion IHstp2_1 as [? [? [? [? [? ?]]]]]; inversion IHstp2_2 as [? [? [? [? [? ?]]]]]; eauto];
-  try solve [inversion IHstp2 as [? [? [? [? [? ?]]]]]; eauto];
-  try solve [inversion IHstp2 as [? [? [? [? [? ?]]]]]; eauto using index_extend].
+  intros G G' x T H HV.
+  induction HV.
+  - assumption.
+  - apply index_extend. apply IHHV. apply H. assumption.
+Qed.
+
+Lemma aenv_ext__same_length:
+  forall GH GH',
+    aenv_ext GH' GH ->
+    length GH = length GH'.
+Proof.
+  intros. induction H.
+  - simpl. reflexivity.
+  - simpl. rewrite IHaenv_ext. reflexivity.
+Qed.
+
+Lemma indexr_at_ext :
+  forall GH GH' x T G,
+    aenv_ext GH' GH ->
+    indexr x GH = Some (G, T) ->
+    exists G', indexr x GH' = Some (G', T) /\ venv_ext G' G.
+Proof.
+  intros GH GH' x T G Hext Hindex. induction Hext.
+  - simpl in Hindex. inversion Hindex.
+  - simpl. simpl in Hindex.
+    case_eq (beq_nat x (length A)); intros E.
+    rewrite E in Hindex.  inversion Hindex. subst.
+    rewrite <- (@aenv_ext__same_length A A'). rewrite E.
+    exists G'. split. reflexivity. assumption. assumption.
+    rewrite E in Hindex.
+    rewrite <- (@aenv_ext__same_length A A'). rewrite E.
+    apply IHHext. assumption. assumption.
+Qed.
+
+Lemma stp2_closure_extend_rec :
+  forall G1 G2 T1 T2 GH,
+    stp2 G1 T1 G2 T2 GH ->
+    (forall G1' G2' GH',
+       aenv_ext GH' GH ->
+       venv_ext G1' G1 ->
+       venv_ext G2' G2 ->
+       stp2 G1' T1 G2' T2 GH').
+Proof.
+  intros G1 G2 T1 T2 GH H.
+  induction H; intros; eauto;
+  try solve [inversion IHstp2_1; inversion IHstp2_2; eauto];
+  try solve [inversion IHstp2; eauto].
+  - Case "sel1".
+    eapply stp2_sel1. eapply index_extend_mult. apply H.
+    assumption. assumption.
+    apply IHstp2. assumption. apply venv_same. assumption.
+  - Case "sel2".
+    eapply stp2_sel2. eapply index_extend_mult. apply H.
+    assumption. assumption.
+    apply IHstp2. assumption. assumption. apply venv_same.
   - Case "sela1".
-    subst. simpl in H.
-    case_eq (beq_nat x (length GH1)); intros E.
-    assert (indexr x (GH0 ++ (x0, (G0, T0)) :: GH1) = Some (G0, T0)) as A. {
-      apply indexr_at_index. assumption.
+    assert (exists GX', indexr x GH' = Some (GX', TX) /\ venv_ext GX' GX) as A. {
+      apply indexr_at_ext with (GH:=GH); assumption.
     }
-    rewrite A in H. inversion H. subst.
-    assert (indexr x (GH0 ++ (x0, ((x1,v1)::GX, TX)) :: GH1) = Some ((x1,v1)::GX, TX)) as A'. {
-      apply indexr_at_index. assumption.
-    }
-    apply stp2_sela1 with (GX:=(x1,v1)::GX) (TX:=TX).
-    simpl. apply A'.
-    inversion IHstp2 as [_ [_ [_ [IH _]]]].
-    apply IH. reflexivity. assumption. assumption.
-    assert (indexr x (GH0 ++ (x0, ((x1,v1)::G0, T0)) :: GH1) = Some (GX, TX)) as A'. {
-      eapply indexr_same. assumption. eassumption.
-    }
-    apply stp2_sela1 with (GX:=GX) (TX:=TX).
-    simpl. rewrite A'. reflexivity.
-    apply IHstp2. reflexivity. assumption.
-  - Case "sela1 (bis)".
-    subst. simpl in H.
-    case_eq (beq_nat x (length GH1)); intros E.
-    assert (indexr x (GH0 ++ (x0, (G0, T0)) :: GH1) = Some (G0, T0)) as A. {
-      apply indexr_at_index. assumption.
-    }
-    rewrite A in H. inversion H. subst.
-    assert (indexr x (GH0 ++ (x0, ((x1,v1)::GX, TX)) :: GH1) = Some ((x1,v1)::GX, TX)) as A'. {
-      apply indexr_at_index. assumption.
-    }
-    apply stp2_sela1 with (GX:=(x1,v1)::GX) (TX:=TX).
-    simpl. apply A'.
-    inversion IHstp2 as [_ [_ [_ [IH _]]]].
-    apply IH. reflexivity. assumption. assumption.
-    assert (indexr x (GH0 ++ (x0, ((x1,v1)::G0, T0)) :: GH1) = Some (GX, TX)) as A'. {
-      eapply indexr_same. assumption. eassumption.
-    }
-    apply stp2_sela1 with (GX:=GX) (TX:=TX).
-    simpl. rewrite A'. reflexivity.
-    apply IHstp2. reflexivity. assumption.
-  - Case "sela1 (bis bis)".
-    subst. simpl in H.
-    case_eq (beq_nat x (length GH1)); intros E.
-    assert (indexr x (GH0 ++ (x0, (G0, T0)) :: GH1) = Some (G0, T0)) as A. {
-      apply indexr_at_index. assumption.
-    }
-    rewrite A in H. inversion H. subst.
-    assert (indexr x (GH0 ++ (x0, ((x1,v1)::GX, TX)) :: GH1) = Some ((x1,v1)::GX, TX)) as A'. {
-      apply indexr_at_index. assumption.
-    }
-    apply stp2_sela1 with (GX:=(x1,v1)::GX) (TX:=TX).
-    simpl. apply A'.
-    inversion IHstp2 as [_ [_ [_ [_ [_ IH]]]]].
-    apply IH. reflexivity. assumption. assumption. assumption.
-    assert (indexr x (GH0 ++ (x0, ((x1,v1)::G0, T0)) :: GH1) = Some (GX, TX)) as A'. {
-      eapply indexr_same. assumption. eassumption.
-    }
-    apply stp2_sela1 with (GX:=GX) (TX:=TX).
-    simpl. rewrite A'. reflexivity.
-    apply IHstp2. reflexivity. assumption. assumption.
-  - Case "sela1 (bis bis bis)".
-    subst. simpl in H.
-    case_eq (beq_nat x (length GH1)); intros E.
-    assert (indexr x (GH0 ++ (x0, (G0, T0)) :: GH1) = Some (G0, T0)) as A. {
-      apply indexr_at_index. assumption.
-    }
-    rewrite A in H. inversion H. subst.
-    assert (indexr x (GH0 ++ (x0, ((x1,v1)::GX, TX)) :: GH1) = Some ((x1,v1)::GX, TX)) as A'. {
-      apply indexr_at_index. assumption.
-    }
-    apply stp2_sela1 with (GX:=(x1,v1)::GX) (TX:=TX).
-    simpl. apply A'.
-    inversion IHstp2 as [_ [_ [_ [_ [_ IH]]]]].
-    apply IH. reflexivity. assumption. assumption. assumption.
-    assert (indexr x (GH0 ++ (x0, ((x1,v1)::G0, T0)) :: GH1) = Some (GX, TX)) as A'. {
-      eapply indexr_same. assumption. eassumption.
-    }
-    apply stp2_sela1 with (GX:=GX) (TX:=TX).
-    simpl. rewrite A'. reflexivity.
-    apply IHstp2. reflexivity. assumption. assumption.
+    inversion A as [GX' [H' HX]].
+    apply stp2_sela1 with (GX:=GX') (TX:=TX).
+    assumption.
+    apply IHstp2; assumption.
   - Case "selax".
-    subst. simpl in H.
-    case_eq (beq_nat x (length GH1)); intros E.
-    assert (indexr x (GH0 ++ (x0, ((x1,v1)::G0, T0)) :: GH1) = Some ((x1,v1)::G0, T0)) as A'. {
-      apply indexr_at_index. assumption.
+    assert (exists GX', indexr x GH' = Some (GX', TX) /\ venv_ext GX' GX) as A. {
+      apply indexr_at_ext with (GH:=GH); assumption.
     }
-    apply stp2_selax with (GX:=(x1,v1)::G0) (TX:=T0).
-    simpl. rewrite A'. simpl. reflexivity. apply A'.
-    assert (indexr x (GH0 ++ (x0, ((x1,v1)::G0, T0)) :: GH1) = Some (GX, TX)) as A'. {
-      eapply indexr_same. assumption. eassumption.
-    }
-    apply stp2_selax with (GX:=GX) (TX:=TX).
-    simpl. apply A'. apply A'.
-  - Case "selax (bis)".
-    subst. simpl in H.
-    case_eq (beq_nat x (length GH1)); intros E.
-    assert (indexr x (GH0 ++ (x0, ((x1,v1)::G0, T0)) :: GH1) = Some ((x1,v1)::G0, T0)) as A'. {
-      apply indexr_at_index. assumption.
-    }
-    apply stp2_selax with (GX:=(x1,v1)::G0) (TX:=T0).
-    simpl. rewrite A'. simpl. reflexivity. apply A'.
-    assert (indexr x (GH0 ++ (x0, ((x1,v1)::G0, T0)) :: GH1) = Some (GX, TX)) as A'. {
-      eapply indexr_same. assumption. eassumption.
-    }
-    apply stp2_selax with (GX:=GX) (TX:=TX).
-    simpl. apply A'. apply A'.
-  - Case "selax (bis bis)".
-    subst. simpl in H.
-    case_eq (beq_nat x (length GH1)); intros E.
-    assert (indexr x (GH0 ++ (x0, ((x1,v1)::G0, T0)) :: GH1) = Some ((x1,v1)::G0, T0)) as A'. {
-      apply indexr_at_index. assumption.
-    }
-    apply stp2_selax with (GX:=(x1,v1)::G0) (TX:=T0).
-    simpl. rewrite A'. simpl. reflexivity. apply A'.
-    assert (indexr x (GH0 ++ (x0, ((x1,v1)::G0, T0)) :: GH1) = Some (GX, TX)) as A'. {
-      eapply indexr_same. assumption. eassumption.
-    }
-    apply stp2_selax with (GX:=GX) (TX:=TX).
-    simpl. apply A'. apply A'.
-  - Case "selax (bis bis bis)".
-    subst. simpl in H.
-    case_eq (beq_nat x (length GH1)); intros E.
-    assert (indexr x (GH0 ++ (x0, ((x1,v1)::G0, T0)) :: GH1) = Some ((x1,v1)::G0, T0)) as A'. {
-      apply indexr_at_index. assumption.
-    }
-    apply stp2_selax with (GX:=(x1,v1)::G0) (TX:=T0).
-    simpl. rewrite A'. simpl. reflexivity. apply A'.
-    assert (indexr x (GH0 ++ (x0, ((x1,v1)::G0, T0)) :: GH1) = Some (GX, TX)) as A'. {
-      eapply indexr_same. assumption. eassumption.
-    }
-    apply stp2_selax with (GX:=GX) (TX:=TX).
-    simpl. apply A'. apply A'.
-  - Case "TAll (extend G2)".
-    inversion IHstp2_1 as [? [? [? [? [? ?]]]]]. inversion IHstp2_2 as [? [? [? [? [? ?]]]]].
-    constructor; eauto. subst.
-    rewrite <- app_nil_l. apply H12. simpl. reflexivity. assumption. assumption.
-  - Case "TAll (refine GH)".
-    assert ((length (GH0 ++ (x0, (G0, T0)) :: GH1))=(length (GH0 ++ (x0, ((x1, v1) :: G0, T0)) :: GH1))) as A. {
-      clear.
-      simpl. induction GH0.
-      - simpl. reflexivity.
-      - simpl. rewrite IHGH0. reflexivity.
+    inversion A as [GX' [H' HX]].
+    apply stp2_selax with (GX:=GX') (TX:=TX).
+    assumption. assumption.
+  - Case "all".
+    assert (length GH = length GH') as A. {
+      apply aenv_ext__same_length. assumption.
     }
     apply stp2_all.
     apply IHstp2_1; assumption.
     subst. rewrite <- A. assumption.
     subst. rewrite <- A. assumption.
     subst. rewrite <- A.
-    change ((0, (G2, T3)) :: GH0 ++ (x0, ((x1, v1) :: G0, T0)) :: GH1) with (((0, (G2, T3)) :: GH0) ++ (x0, ((x1, v1) :: G0, T0)) :: GH1).
-    apply IHstp2_2.
-    simpl. reflexivity. assumption.
-  - Case "TAll (refine GH bis)".
-    assert ((length (GH0 ++ (x0, (G0, T0)) :: GH1))=(length (GH0 ++ (x0, ((x1, v1) :: G0, T0)) :: GH1))) as A. {
-      clear.
-      simpl. induction GH0.
-      - simpl. reflexivity.
-      - simpl. rewrite IHGH0. reflexivity.
-    }
-    apply stp2_all.
-    apply IHstp2_1; assumption.
-    subst. rewrite <- A. assumption.
-    subst. rewrite <- A. assumption.
-    subst. rewrite <- A.
-    change ((0, (G2, T3)) :: GH0 ++ (x0, ((x1, v1) :: G0, T0)) :: GH1) with (((0, (G2, T3)) :: GH0) ++ (x0, ((x1, v1) :: G0, T0)) :: GH1).
-    apply IHstp2_2.
-    simpl. reflexivity. assumption. assumption.
-  - Case "TAll (refine GH bis bis)".
-    assert ((length (GH0 ++ (x0, (G0, T0)) :: GH1))=(length (GH0 ++ (x0, ((x1, v1) :: G0, T0)) :: GH1))) as A. {
-      clear.
-      simpl. induction GH0.
-      - simpl. reflexivity.
-      - simpl. rewrite IHGH0. reflexivity.
-    }
-    apply stp2_all.
-    apply IHstp2_1; assumption.
-    subst. rewrite <- A. assumption.
-    subst. rewrite <- A. assumption.
-    subst. rewrite <- A.
-    rewrite <- app_nil_l.
-    apply IHstp2_2. simpl. admit. assumption. assumption.
-  - Case "TAll (refine GH bis bis bis)".
-    assert ((length (GH0 ++ (x0, (G0, T0)) :: GH1))=(length (GH0 ++ (x0, ((x1, v1) :: G0, T0)) :: GH1))) as A. {
-      clear.
-      simpl. induction GH0.
-      - simpl. reflexivity.
-      - simpl. rewrite IHGH0. reflexivity.
-    }
-    apply stp2_all.
-    apply IHstp2_1; assumption.
-    subst. rewrite <- A. assumption.
-    subst. rewrite <- A. assumption.
-    subst. rewrite <- A.
-    rewrite <- app_nil_l.
-    apply IHstp2_2. simpl. admit. assumption. assumption. assumption.
+    apply IHstp2_2. apply aenv_cons. assumption. assumption. assumption. assumption.
 Qed.
 
 
